{
 "cells": [
  {
   "cell_type": "code",
   "execution_count": 2,
   "id": "8717e83f-8793-45a4-8cc0-228e60917acd",
   "metadata": {},
   "outputs": [
    {
     "data": {
      "text/plain": [
       "cofactor (generic function with 3 methods)"
      ]
     },
     "metadata": {},
     "output_type": "display_data"
    }
   ],
   "source": [
    "include(\"main_whit.jl\")"
   ]
  },
  {
   "cell_type": "code",
   "execution_count": 3,
   "id": "0b3d0446-5bf2-494d-9a96-efa5b7ee07ad",
   "metadata": {},
   "outputs": [
    {
     "data": {
      "text/latex": [
       "$$ \\begin{equation}\n",
       "\\left[\n",
       "\\begin{array}{cccccc}\n",
       "w_1 + \\lambda &  - 2 \\lambda & \\lambda & 0 & 0 & 0 \\\\\n",
       " - 2 \\lambda & w_2 + 5 \\lambda &  - 4 \\lambda & \\lambda & 0 & 0 \\\\\n",
       "\\lambda &  - 4 \\lambda & w_3 + 6 \\lambda &  - 4 \\lambda & \\lambda & 0 \\\\\n",
       "0 & \\lambda &  - 4 \\lambda & w_4 + 6 \\lambda &  - 4 \\lambda & \\lambda \\\\\n",
       "0 & 0 & \\lambda &  - 4 \\lambda & w_5 + 5 \\lambda &  - 2 \\lambda \\\\\n",
       "0 & 0 & 0 & \\lambda &  - 2 \\lambda & w_6 + \\lambda \\\\\n",
       "\\end{array}\n",
       "\\right]\n",
       "\\end{equation}\n",
       " $$"
      ],
      "text/plain": [
       "6×6 Matrix{Num}:\n",
       " w₁ + λ        -2λ          λ          0.0        0.0       0.0\n",
       "    -2λ    w₂ + 5λ        -4λ          λ          0.0       0.0\n",
       "      λ        -4λ    w₃ + 6λ        -4λ          λ         0.0\n",
       "      0.0        λ        -4λ    w₄ + 6λ        -4λ         λ\n",
       "      0.0        0.0        λ        -4λ    w₅ + 5λ       -2λ\n",
       "      0.0        0.0        0.0        λ        -2λ    w₆ + λ"
      ]
     },
     "metadata": {},
     "output_type": "display_data"
    },
    {
     "data": {
      "text/latex": [
       "$$ \\begin{equation}\n",
       "\\left[\n",
       "\\begin{array}{cccccc}\n",
       "1 & 0 & 0 & 0 & 0 & 0 \\\\\n",
       "\\frac{ - 2 \\lambda}{w_1 + \\lambda} & 1 & 0 & 0 & 0 & 0 \\\\\n",
       "\\frac{\\lambda}{w_1 + \\lambda} & \\frac{\\frac{2 \\lambda^{2}}{w_1 + \\lambda} - 4 \\lambda}{w_2 + \\frac{ - 4 \\lambda^{2}}{w_1 + \\lambda} + 5 \\lambda} & 1 & 0 & 0 & 0 \\\\\n",
       "0 & \\frac{\\lambda}{w_2 + \\frac{ - 4 \\lambda^{2}}{w_1 + \\lambda} + 5 \\lambda} & \\frac{\\frac{ - \\left( \\frac{2 \\lambda^{2}}{w_1 + \\lambda} - 4 \\lambda \\right) \\lambda}{w_2 + \\frac{ - 4 \\lambda^{2}}{w_1 + \\lambda} + 5 \\lambda} - 4 \\lambda}{w_3 + \\frac{ - \\left( \\frac{2 \\lambda^{2}}{w_1 + \\lambda} - 4 \\lambda \\right)^{2}}{w_2 + \\frac{ - 4 \\lambda^{2}}{w_1 + \\lambda} + 5 \\lambda} + \\frac{ - \\lambda^{2}}{w_1 + \\lambda} + 6 \\lambda} & 1 & 0 & 0 \\\\\n",
       "0 & 0 & \\frac{\\lambda}{w_3 + \\frac{ - \\left( \\frac{2 \\lambda^{2}}{w_1 + \\lambda} - 4 \\lambda \\right)^{2}}{w_2 + \\frac{ - 4 \\lambda^{2}}{w_1 + \\lambda} + 5 \\lambda} + \\frac{ - \\lambda^{2}}{w_1 + \\lambda} + 6 \\lambda} & \\frac{\\frac{ - \\left( \\frac{ - \\left( \\frac{2 \\lambda^{2}}{w_1 + \\lambda} - 4 \\lambda \\right) \\lambda}{w_2 + \\frac{ - 4 \\lambda^{2}}{w_1 + \\lambda} + 5 \\lambda} - 4 \\lambda \\right) \\lambda}{w_3 + \\frac{ - \\left( \\frac{2 \\lambda^{2}}{w_1 + \\lambda} - 4 \\lambda \\right)^{2}}{w_2 + \\frac{ - 4 \\lambda^{2}}{w_1 + \\lambda} + 5 \\lambda} + \\frac{ - \\lambda^{2}}{w_1 + \\lambda} + 6 \\lambda} - 4 \\lambda}{w_4 + \\frac{ - \\left( \\frac{ - \\left( \\frac{2 \\lambda^{2}}{w_1 + \\lambda} - 4 \\lambda \\right) \\lambda}{w_2 + \\frac{ - 4 \\lambda^{2}}{w_1 + \\lambda} + 5 \\lambda} - 4 \\lambda \\right)^{2}}{w_3 + \\frac{ - \\left( \\frac{2 \\lambda^{2}}{w_1 + \\lambda} - 4 \\lambda \\right)^{2}}{w_2 + \\frac{ - 4 \\lambda^{2}}{w_1 + \\lambda} + 5 \\lambda} + \\frac{ - \\lambda^{2}}{w_1 + \\lambda} + 6 \\lambda} + \\frac{ - \\lambda^{2}}{w_2 + \\frac{ - 4 \\lambda^{2}}{w_1 + \\lambda} + 5 \\lambda} + 6 \\lambda} & 1 & 0 \\\\\n",
       "0 & 0 & 0 & \\frac{\\lambda}{w_4 + \\frac{ - \\left( \\frac{ - \\left( \\frac{2 \\lambda^{2}}{w_1 + \\lambda} - 4 \\lambda \\right) \\lambda}{w_2 + \\frac{ - 4 \\lambda^{2}}{w_1 + \\lambda} + 5 \\lambda} - 4 \\lambda \\right)^{2}}{w_3 + \\frac{ - \\left( \\frac{2 \\lambda^{2}}{w_1 + \\lambda} - 4 \\lambda \\right)^{2}}{w_2 + \\frac{ - 4 \\lambda^{2}}{w_1 + \\lambda} + 5 \\lambda} + \\frac{ - \\lambda^{2}}{w_1 + \\lambda} + 6 \\lambda} + \\frac{ - \\lambda^{2}}{w_2 + \\frac{ - 4 \\lambda^{2}}{w_1 + \\lambda} + 5 \\lambda} + 6 \\lambda} & \\frac{\\frac{ - \\left( \\frac{ - \\left( \\frac{ - \\left( \\frac{2 \\lambda^{2}}{w_1 + \\lambda} - 4 \\lambda \\right) \\lambda}{w_2 + \\frac{ - 4 \\lambda^{2}}{w_1 + \\lambda} + 5 \\lambda} - 4 \\lambda \\right) \\lambda}{w_3 + \\frac{ - \\left( \\frac{2 \\lambda^{2}}{w_1 + \\lambda} - 4 \\lambda \\right)^{2}}{w_2 + \\frac{ - 4 \\lambda^{2}}{w_1 + \\lambda} + 5 \\lambda} + \\frac{ - \\lambda^{2}}{w_1 + \\lambda} + 6 \\lambda} - 4 \\lambda \\right) \\lambda}{w_4 + \\frac{ - \\left( \\frac{ - \\left( \\frac{2 \\lambda^{2}}{w_1 + \\lambda} - 4 \\lambda \\right) \\lambda}{w_2 + \\frac{ - 4 \\lambda^{2}}{w_1 + \\lambda} + 5 \\lambda} - 4 \\lambda \\right)^{2}}{w_3 + \\frac{ - \\left( \\frac{2 \\lambda^{2}}{w_1 + \\lambda} - 4 \\lambda \\right)^{2}}{w_2 + \\frac{ - 4 \\lambda^{2}}{w_1 + \\lambda} + 5 \\lambda} + \\frac{ - \\lambda^{2}}{w_1 + \\lambda} + 6 \\lambda} + \\frac{ - \\lambda^{2}}{w_2 + \\frac{ - 4 \\lambda^{2}}{w_1 + \\lambda} + 5 \\lambda} + 6 \\lambda} - 2 \\lambda}{w_5 + \\frac{ - \\left( \\frac{ - \\left( \\frac{ - \\left( \\frac{2 \\lambda^{2}}{w_1 + \\lambda} - 4 \\lambda \\right) \\lambda}{w_2 + \\frac{ - 4 \\lambda^{2}}{w_1 + \\lambda} + 5 \\lambda} - 4 \\lambda \\right) \\lambda}{w_3 + \\frac{ - \\left( \\frac{2 \\lambda^{2}}{w_1 + \\lambda} - 4 \\lambda \\right)^{2}}{w_2 + \\frac{ - 4 \\lambda^{2}}{w_1 + \\lambda} + 5 \\lambda} + \\frac{ - \\lambda^{2}}{w_1 + \\lambda} + 6 \\lambda} - 4 \\lambda \\right)^{2}}{w_4 + \\frac{ - \\left( \\frac{ - \\left( \\frac{2 \\lambda^{2}}{w_1 + \\lambda} - 4 \\lambda \\right) \\lambda}{w_2 + \\frac{ - 4 \\lambda^{2}}{w_1 + \\lambda} + 5 \\lambda} - 4 \\lambda \\right)^{2}}{w_3 + \\frac{ - \\left( \\frac{2 \\lambda^{2}}{w_1 + \\lambda} - 4 \\lambda \\right)^{2}}{w_2 + \\frac{ - 4 \\lambda^{2}}{w_1 + \\lambda} + 5 \\lambda} + \\frac{ - \\lambda^{2}}{w_1 + \\lambda} + 6 \\lambda} + \\frac{ - \\lambda^{2}}{w_2 + \\frac{ - 4 \\lambda^{2}}{w_1 + \\lambda} + 5 \\lambda} + 6 \\lambda} + \\frac{ - \\lambda^{2}}{w_3 + \\frac{ - \\left( \\frac{2 \\lambda^{2}}{w_1 + \\lambda} - 4 \\lambda \\right)^{2}}{w_2 + \\frac{ - 4 \\lambda^{2}}{w_1 + \\lambda} + 5 \\lambda} + \\frac{ - \\lambda^{2}}{w_1 + \\lambda} + 6 \\lambda} + 5 \\lambda} & 1 \\\\\n",
       "\\end{array}\n",
       "\\right]\n",
       "\\end{equation}\n",
       " $$"
      ],
      "text/plain": [
       "6×6 Matrix{Num}:\n",
       "                1    …  0\n",
       " (-2λ) / (w₁ + λ)       0\n",
       "     λ / (w₁ + λ)       0\n",
       "                0.0     0\n",
       "                0.0     0\n",
       "                0.0  …  1"
      ]
     },
     "metadata": {},
     "output_type": "display_data"
    }
   ],
   "source": [
    "n = 6\n",
    "w = variables(:w, 1:n)\n",
    "D = ddmat(1:n, 2)\n",
    "# M = diagm(ones(n))\n",
    "M = diag_m(w[1:n]) + λ * D' * D\n",
    "display(M)\n",
    "# M = diagm(W) + λ * D' * D\n",
    "\n",
    "U = deepcopy(M)\n",
    "L = typeof(U)(diagm(ones(n)))\n",
    "\n",
    "r = lu(M)\n",
    "## lu采用for循环的形式，\n",
    "r.L"
   ]
  },
  {
   "cell_type": "code",
   "execution_count": 7,
   "id": "51947888-a1e3-4ade-9df4-dc4caeb2add2",
   "metadata": {},
   "outputs": [
    {
     "data": {
      "text/latex": [
       "$$ \\begin{equation}\n",
       "\\left[\n",
       "\\begin{array}{cccccc}\n",
       "w_{1} + \\lambda &  - 2 \\lambda & \\lambda & 0 & 0 & 0 \\\\\n",
       "0 & w_{2} + \\frac{ - 4 \\lambda^{2}}{w_{1} + \\lambda} + 5 \\lambda & \\frac{2 \\lambda^{2}}{w_{1} + \\lambda} - 4 \\lambda & \\lambda & 0 & 0 \\\\\n",
       "0 & 0 & w_{3} + \\frac{ - \\lambda^{2}}{w_{1} + \\lambda} + \\frac{ - \\left( \\frac{2 \\lambda^{2}}{w_{1} + \\lambda} - 4 \\lambda \\right)^{2}}{w_{2} + \\frac{ - 4 \\lambda^{2}}{w_{1} + \\lambda} + 5 \\lambda} + 6 \\lambda & \\frac{ - \\left( \\frac{2 \\lambda^{2}}{w_{1} + \\lambda} - 4 \\lambda \\right) \\lambda}{w_{2} + \\frac{ - 4 \\lambda^{2}}{w_{1} + \\lambda} + 5 \\lambda} - 4 \\lambda & \\lambda & 0 \\\\\n",
       "0 & 0 & 0 & w_{4} + \\frac{ - \\left( \\frac{ - \\left( \\frac{2 \\lambda^{2}}{w_{1} + \\lambda} - 4 \\lambda \\right) \\lambda}{w_{2} + \\frac{ - 4 \\lambda^{2}}{w_{1} + \\lambda} + 5 \\lambda} - 4 \\lambda \\right)^{2}}{w_{3} + \\frac{ - \\lambda^{2}}{w_{1} + \\lambda} + \\frac{ - \\left( \\frac{2 \\lambda^{2}}{w_{1} + \\lambda} - 4 \\lambda \\right)^{2}}{w_{2} + \\frac{ - 4 \\lambda^{2}}{w_{1} + \\lambda} + 5 \\lambda} + 6 \\lambda} + \\frac{ - \\lambda^{2}}{w_{2} + \\frac{ - 4 \\lambda^{2}}{w_{1} + \\lambda} + 5 \\lambda} + 6 \\lambda & \\frac{ - \\left( \\frac{ - \\left( \\frac{2 \\lambda^{2}}{w_{1} + \\lambda} - 4 \\lambda \\right) \\lambda}{w_{2} + \\frac{ - 4 \\lambda^{2}}{w_{1} + \\lambda} + 5 \\lambda} - 4 \\lambda \\right) \\lambda}{w_{3} + \\frac{ - \\lambda^{2}}{w_{1} + \\lambda} + \\frac{ - \\left( \\frac{2 \\lambda^{2}}{w_{1} + \\lambda} - 4 \\lambda \\right)^{2}}{w_{2} + \\frac{ - 4 \\lambda^{2}}{w_{1} + \\lambda} + 5 \\lambda} + 6 \\lambda} - 4 \\lambda & \\lambda \\\\\n",
       "0 & 0 & 0 & 0 & w_{5} + \\frac{ - \\left( \\frac{ - \\left( \\frac{ - \\left( \\frac{2 \\lambda^{2}}{w_{1} + \\lambda} - 4 \\lambda \\right) \\lambda}{w_{2} + \\frac{ - 4 \\lambda^{2}}{w_{1} + \\lambda} + 5 \\lambda} - 4 \\lambda \\right) \\lambda}{w_{3} + \\frac{ - \\lambda^{2}}{w_{1} + \\lambda} + \\frac{ - \\left( \\frac{2 \\lambda^{2}}{w_{1} + \\lambda} - 4 \\lambda \\right)^{2}}{w_{2} + \\frac{ - 4 \\lambda^{2}}{w_{1} + \\lambda} + 5 \\lambda} + 6 \\lambda} - 4 \\lambda \\right)^{2}}{w_{4} + \\frac{ - \\left( \\frac{ - \\left( \\frac{2 \\lambda^{2}}{w_{1} + \\lambda} - 4 \\lambda \\right) \\lambda}{w_{2} + \\frac{ - 4 \\lambda^{2}}{w_{1} + \\lambda} + 5 \\lambda} - 4 \\lambda \\right)^{2}}{w_{3} + \\frac{ - \\lambda^{2}}{w_{1} + \\lambda} + \\frac{ - \\left( \\frac{2 \\lambda^{2}}{w_{1} + \\lambda} - 4 \\lambda \\right)^{2}}{w_{2} + \\frac{ - 4 \\lambda^{2}}{w_{1} + \\lambda} + 5 \\lambda} + 6 \\lambda} + \\frac{ - \\lambda^{2}}{w_{2} + \\frac{ - 4 \\lambda^{2}}{w_{1} + \\lambda} + 5 \\lambda} + 6 \\lambda} + \\frac{ - \\lambda^{2}}{w_{3} + \\frac{ - \\lambda^{2}}{w_{1} + \\lambda} + \\frac{ - \\left( \\frac{2 \\lambda^{2}}{w_{1} + \\lambda} - 4 \\lambda \\right)^{2}}{w_{2} + \\frac{ - 4 \\lambda^{2}}{w_{1} + \\lambda} + 5 \\lambda} + 6 \\lambda} + 5 \\lambda & \\frac{ - \\left( \\frac{ - \\left( \\frac{ - \\left( \\frac{2 \\lambda^{2}}{w_{1} + \\lambda} - 4 \\lambda \\right) \\lambda}{w_{2} + \\frac{ - 4 \\lambda^{2}}{w_{1} + \\lambda} + 5 \\lambda} - 4 \\lambda \\right) \\lambda}{w_{3} + \\frac{ - \\lambda^{2}}{w_{1} + \\lambda} + \\frac{ - \\left( \\frac{2 \\lambda^{2}}{w_{1} + \\lambda} - 4 \\lambda \\right)^{2}}{w_{2} + \\frac{ - 4 \\lambda^{2}}{w_{1} + \\lambda} + 5 \\lambda} + 6 \\lambda} - 4 \\lambda \\right) \\lambda}{w_{4} + \\frac{ - \\left( \\frac{ - \\left( \\frac{2 \\lambda^{2}}{w_{1} + \\lambda} - 4 \\lambda \\right) \\lambda}{w_{2} + \\frac{ - 4 \\lambda^{2}}{w_{1} + \\lambda} + 5 \\lambda} - 4 \\lambda \\right)^{2}}{w_{3} + \\frac{ - \\lambda^{2}}{w_{1} + \\lambda} + \\frac{ - \\left( \\frac{2 \\lambda^{2}}{w_{1} + \\lambda} - 4 \\lambda \\right)^{2}}{w_{2} + \\frac{ - 4 \\lambda^{2}}{w_{1} + \\lambda} + 5 \\lambda} + 6 \\lambda} + \\frac{ - \\lambda^{2}}{w_{2} + \\frac{ - 4 \\lambda^{2}}{w_{1} + \\lambda} + 5 \\lambda} + 6 \\lambda} - 2 \\lambda \\\\\n",
       "0 & 0 & 0 & 0 & 0 & w_{6} + \\frac{ - \\left( \\frac{ - \\left( \\frac{ - \\left( \\frac{ - \\left( \\frac{2 \\lambda^{2}}{w_{1} + \\lambda} - 4 \\lambda \\right) \\lambda}{w_{2} + \\frac{ - 4 \\lambda^{2}}{w_{1} + \\lambda} + 5 \\lambda} - 4 \\lambda \\right) \\lambda}{w_{3} + \\frac{ - \\lambda^{2}}{w_{1} + \\lambda} + \\frac{ - \\left( \\frac{2 \\lambda^{2}}{w_{1} + \\lambda} - 4 \\lambda \\right)^{2}}{w_{2} + \\frac{ - 4 \\lambda^{2}}{w_{1} + \\lambda} + 5 \\lambda} + 6 \\lambda} - 4 \\lambda \\right) \\lambda}{w_{4} + \\frac{ - \\left( \\frac{ - \\left( \\frac{2 \\lambda^{2}}{w_{1} + \\lambda} - 4 \\lambda \\right) \\lambda}{w_{2} + \\frac{ - 4 \\lambda^{2}}{w_{1} + \\lambda} + 5 \\lambda} - 4 \\lambda \\right)^{2}}{w_{3} + \\frac{ - \\lambda^{2}}{w_{1} + \\lambda} + \\frac{ - \\left( \\frac{2 \\lambda^{2}}{w_{1} + \\lambda} - 4 \\lambda \\right)^{2}}{w_{2} + \\frac{ - 4 \\lambda^{2}}{w_{1} + \\lambda} + 5 \\lambda} + 6 \\lambda} + \\frac{ - \\lambda^{2}}{w_{2} + \\frac{ - 4 \\lambda^{2}}{w_{1} + \\lambda} + 5 \\lambda} + 6 \\lambda} - 2 \\lambda \\right)^{2}}{w_{5} + \\frac{ - \\left( \\frac{ - \\left( \\frac{ - \\left( \\frac{2 \\lambda^{2}}{w_{1} + \\lambda} - 4 \\lambda \\right) \\lambda}{w_{2} + \\frac{ - 4 \\lambda^{2}}{w_{1} + \\lambda} + 5 \\lambda} - 4 \\lambda \\right) \\lambda}{w_{3} + \\frac{ - \\lambda^{2}}{w_{1} + \\lambda} + \\frac{ - \\left( \\frac{2 \\lambda^{2}}{w_{1} + \\lambda} - 4 \\lambda \\right)^{2}}{w_{2} + \\frac{ - 4 \\lambda^{2}}{w_{1} + \\lambda} + 5 \\lambda} + 6 \\lambda} - 4 \\lambda \\right)^{2}}{w_{4} + \\frac{ - \\left( \\frac{ - \\left( \\frac{2 \\lambda^{2}}{w_{1} + \\lambda} - 4 \\lambda \\right) \\lambda}{w_{2} + \\frac{ - 4 \\lambda^{2}}{w_{1} + \\lambda} + 5 \\lambda} - 4 \\lambda \\right)^{2}}{w_{3} + \\frac{ - \\lambda^{2}}{w_{1} + \\lambda} + \\frac{ - \\left( \\frac{2 \\lambda^{2}}{w_{1} + \\lambda} - 4 \\lambda \\right)^{2}}{w_{2} + \\frac{ - 4 \\lambda^{2}}{w_{1} + \\lambda} + 5 \\lambda} + 6 \\lambda} + \\frac{ - \\lambda^{2}}{w_{2} + \\frac{ - 4 \\lambda^{2}}{w_{1} + \\lambda} + 5 \\lambda} + 6 \\lambda} + \\frac{ - \\lambda^{2}}{w_{3} + \\frac{ - \\lambda^{2}}{w_{1} + \\lambda} + \\frac{ - \\left( \\frac{2 \\lambda^{2}}{w_{1} + \\lambda} - 4 \\lambda \\right)^{2}}{w_{2} + \\frac{ - 4 \\lambda^{2}}{w_{1} + \\lambda} + 5 \\lambda} + 6 \\lambda} + 5 \\lambda} + \\frac{ - \\lambda^{2}}{w_{4} + \\frac{ - \\left( \\frac{ - \\left( \\frac{2 \\lambda^{2}}{w_{1} + \\lambda} - 4 \\lambda \\right) \\lambda}{w_{2} + \\frac{ - 4 \\lambda^{2}}{w_{1} + \\lambda} + 5 \\lambda} - 4 \\lambda \\right)^{2}}{w_{3} + \\frac{ - \\lambda^{2}}{w_{1} + \\lambda} + \\frac{ - \\left( \\frac{2 \\lambda^{2}}{w_{1} + \\lambda} - 4 \\lambda \\right)^{2}}{w_{2} + \\frac{ - 4 \\lambda^{2}}{w_{1} + \\lambda} + 5 \\lambda} + 6 \\lambda} + \\frac{ - \\lambda^{2}}{w_{2} + \\frac{ - 4 \\lambda^{2}}{w_{1} + \\lambda} + 5 \\lambda} + 6 \\lambda} + \\lambda \\\\\n",
       "\\end{array}\n",
       "\\right]\n",
       "\\end{equation}\n",
       " $$"
      ],
      "text/plain": [
       "6×6 Matrix{Num}:\n",
       " w_1 + λ  …                                                                                                                                                                                                                                                                                                                                                                                                                                                                                                                                                                                                                                                                                                                                                                                                                                                                                                                                                                                                                                                                                                                                                                                                                                                                                                                                                                                                        0.0\n",
       "       0                                                                                                                                                                                                                                                                                                                                                                                                                                                                                                                                                                                                                                                                                                                                                                                                                                                                                                                                                                                                                                                                                                                                                                                                                                                                                                                                                                                                           0.0\n",
       "       0                                                                                                                                                                                                                                                                                                                                                                                                                                                                                                                                                                                                                                                                                                                                                                                                                                                                                                                                                                                                                                                                                                                                                                                                                                                                                                                                                                                                           0.0\n",
       "       0                                                                                                                                                                                                                                                                                                                                                                                                                                                                                                                                                                                                                                                                                                                                                                                                                                                                                                                                                                                                                                                                                                                                                                                                                                                                                                                                                                                                           λ\n",
       "       0                                                                                                                                                                                                                                                                                                                                                                                                                                                                                                                                                                                                                                                                                                                                                                                                                                                                                                                           (-((-((-((2(λ^2)) / (w_1 + λ) - 4λ)*λ) / (w_2 + (-4(λ^2)) / (w_1 + λ) + 5λ) - 4λ)*λ) / (w_3 + (-(λ^2)) / (w_1 + λ) + (-(((2(λ^2)) / (w_1 + λ) - 4λ)^2)) / (w_2 + (-4(λ^2)) / (w_1 + λ) + 5λ) + 6λ) - 4λ)*λ) / (w_4 + (-(((-((2(λ^2)) / (w_1 + λ) - 4λ)*λ) / (w_2 + (-4(λ^2)) / (w_1 + λ) + 5λ) - 4λ)^2)) / (w_3 + (-(λ^2)) / (w_1 + λ) + (-(((2(λ^2)) / (w_1 + λ) - 4λ)^2)) / (w_2 + (-4(λ^2)) / (w_1 + λ) + 5λ) + 6λ) + (-(λ^2)) / (w_2 + (-4(λ^2)) / (w_1 + λ) + 5λ) + 6λ) - 2λ\n",
       "       0  …  w_6 + (-(((-((-((-((2(λ^2)) / (w_1 + λ) - 4λ)*λ) / (w_2 + (-4(λ^2)) / (w_1 + λ) + 5λ) - 4λ)*λ) / (w_3 + (-(λ^2)) / (w_1 + λ) + (-(((2(λ^2)) / (w_1 + λ) - 4λ)^2)) / (w_2 + (-4(λ^2)) / (w_1 + λ) + 5λ) + 6λ) - 4λ)*λ) / (w_4 + (-(((-((2(λ^2)) / (w_1 + λ) - 4λ)*λ) / (w_2 + (-4(λ^2)) / (w_1 + λ) + 5λ) - 4λ)^2)) / (w_3 + (-(λ^2)) / (w_1 + λ) + (-(((2(λ^2)) / (w_1 + λ) - 4λ)^2)) / (w_2 + (-4(λ^2)) / (w_1 + λ) + 5λ) + 6λ) + (-(λ^2)) / (w_2 + (-4(λ^2)) / (w_1 + λ) + 5λ) + 6λ) - 2λ)^2)) / (w_5 + (-(((-((-((2(λ^2)) / (w_1 + λ) - 4λ)*λ) / (w_2 + (-4(λ^2)) / (w_1 + λ) + 5λ) - 4λ)*λ) / (w_3 + (-(λ^2)) / (w_1 + λ) + (-(((2(λ^2)) / (w_1 + λ) - 4λ)^2)) / (w_2 + (-4(λ^2)) / (w_1 + λ) + 5λ) + 6λ) - 4λ)^2)) / (w_4 + (-(((-((2(λ^2)) / (w_1 + λ) - 4λ)*λ) / (w_2 + (-4(λ^2)) / (w_1 + λ) + 5λ) - 4λ)^2)) / (w_3 + (-(λ^2)) / (w_1 + λ) + (-(((2(λ^2)) / (w_1 + λ) - 4λ)^2)) / (w_2 + (-4(λ^2)) / (w_1 + λ) + 5λ) + 6λ) + (-(λ^2)) / (w_2 + (-4(λ^2)) / (w_1 + λ) + 5λ) + 6λ) + (-(λ^2)) / (w_3 + (-(λ^2)) / (w_1 + λ) + (-(((2(λ^2)) / (w_1 + λ) - 4λ)^2)) / (w_2 + (-4(λ^2)) / (w_1 + λ) + 5λ) + 6λ) + 5λ) + (-(λ^2)) / (w_4 + (-(((-((2(λ^2)) / (w_1 + λ) - 4λ)*λ) / (w_2 + (-4(λ^2)) / (w_1 + λ) + 5λ) - 4λ)^2)) / (w_3 + (-(λ^2)) / (w_1 + λ) + (-(((2(λ^2)) / (w_1 + λ) - 4λ)^2)) / (w_2 + (-4(λ^2)) / (w_1 + λ) + 5λ) + 6λ) + (-(λ^2)) / (w_2 + (-4(λ^2)) / (w_1 + λ) + 5λ) + 6λ) + λ"
      ]
     },
     "execution_count": 7,
     "metadata": {},
     "output_type": "execute_result"
    }
   ],
   "source": [
    "r.U"
   ]
  },
  {
   "cell_type": "code",
   "execution_count": null,
   "id": "c80fd687-a0d6-4f73-8e6d-cb4158065161",
   "metadata": {},
   "outputs": [],
   "source": []
  },
  {
   "cell_type": "code",
   "execution_count": 11,
   "id": "709c66c6-8ba1-40d5-8d5b-7021c64e0cb7",
   "metadata": {},
   "outputs": [
    {
     "data": {
      "text/latex": [
       "$$ \\begin{equation}\n",
       "\\left[\n",
       "\\begin{array}{cccccccc}\n",
       "1 & 0 & 0 & 0 & 0 & 0 & 0 & 0 \\\\\n",
       "\\frac{ - 2 \\lambda}{1 + \\lambda} & 1 & 0 & 0 & 0 & 0 & 0 & 0 \\\\\n",
       "\\frac{\\lambda}{1 + \\lambda} & \\frac{\\frac{2 \\lambda^{2}}{1 + \\lambda} - 4 \\lambda}{1 + \\frac{ - 4 \\lambda^{2}}{1 + \\lambda} + 5 \\lambda} & 1 & 0 & 0 & 0 & 0 & 0 \\\\\n",
       "0 & \\frac{\\lambda}{1 + \\frac{ - 4 \\lambda^{2}}{1 + \\lambda} + 5 \\lambda} & \\frac{\\frac{ - \\left( \\frac{2 \\lambda^{2}}{1 + \\lambda} - 4 \\lambda \\right) \\lambda}{1 + \\frac{ - 4 \\lambda^{2}}{1 + \\lambda} + 5 \\lambda} - 4 \\lambda}{1 + \\frac{ - \\left( \\frac{2 \\lambda^{2}}{1 + \\lambda} - 4 \\lambda \\right)^{2}}{1 + \\frac{ - 4 \\lambda^{2}}{1 + \\lambda} + 5 \\lambda} + \\frac{ - \\lambda^{2}}{1 + \\lambda} + 6 \\lambda} & 1 & 0 & 0 & 0 & 0 \\\\\n",
       "0 & 0 & \\frac{\\lambda}{1 + \\frac{ - \\left( \\frac{2 \\lambda^{2}}{1 + \\lambda} - 4 \\lambda \\right)^{2}}{1 + \\frac{ - 4 \\lambda^{2}}{1 + \\lambda} + 5 \\lambda} + \\frac{ - \\lambda^{2}}{1 + \\lambda} + 6 \\lambda} & \\frac{\\frac{ - \\left( \\frac{ - \\left( \\frac{2 \\lambda^{2}}{1 + \\lambda} - 4 \\lambda \\right) \\lambda}{1 + \\frac{ - 4 \\lambda^{2}}{1 + \\lambda} + 5 \\lambda} - 4 \\lambda \\right) \\lambda}{1 + \\frac{ - \\left( \\frac{2 \\lambda^{2}}{1 + \\lambda} - 4 \\lambda \\right)^{2}}{1 + \\frac{ - 4 \\lambda^{2}}{1 + \\lambda} + 5 \\lambda} + \\frac{ - \\lambda^{2}}{1 + \\lambda} + 6 \\lambda} - 4 \\lambda}{1 + \\frac{ - \\lambda^{2}}{1 + \\frac{ - 4 \\lambda^{2}}{1 + \\lambda} + 5 \\lambda} + \\frac{ - \\left( \\frac{ - \\left( \\frac{2 \\lambda^{2}}{1 + \\lambda} - 4 \\lambda \\right) \\lambda}{1 + \\frac{ - 4 \\lambda^{2}}{1 + \\lambda} + 5 \\lambda} - 4 \\lambda \\right)^{2}}{1 + \\frac{ - \\left( \\frac{2 \\lambda^{2}}{1 + \\lambda} - 4 \\lambda \\right)^{2}}{1 + \\frac{ - 4 \\lambda^{2}}{1 + \\lambda} + 5 \\lambda} + \\frac{ - \\lambda^{2}}{1 + \\lambda} + 6 \\lambda} + 6 \\lambda} & 1 & 0 & 0 & 0 \\\\\n",
       "0 & 0 & 0 & \\frac{\\lambda}{1 + \\frac{ - \\lambda^{2}}{1 + \\frac{ - 4 \\lambda^{2}}{1 + \\lambda} + 5 \\lambda} + \\frac{ - \\left( \\frac{ - \\left( \\frac{2 \\lambda^{2}}{1 + \\lambda} - 4 \\lambda \\right) \\lambda}{1 + \\frac{ - 4 \\lambda^{2}}{1 + \\lambda} + 5 \\lambda} - 4 \\lambda \\right)^{2}}{1 + \\frac{ - \\left( \\frac{2 \\lambda^{2}}{1 + \\lambda} - 4 \\lambda \\right)^{2}}{1 + \\frac{ - 4 \\lambda^{2}}{1 + \\lambda} + 5 \\lambda} + \\frac{ - \\lambda^{2}}{1 + \\lambda} + 6 \\lambda} + 6 \\lambda} & \\frac{\\frac{ - \\left( \\frac{ - \\left( \\frac{ - \\left( \\frac{2 \\lambda^{2}}{1 + \\lambda} - 4 \\lambda \\right) \\lambda}{1 + \\frac{ - 4 \\lambda^{2}}{1 + \\lambda} + 5 \\lambda} - 4 \\lambda \\right) \\lambda}{1 + \\frac{ - \\left( \\frac{2 \\lambda^{2}}{1 + \\lambda} - 4 \\lambda \\right)^{2}}{1 + \\frac{ - 4 \\lambda^{2}}{1 + \\lambda} + 5 \\lambda} + \\frac{ - \\lambda^{2}}{1 + \\lambda} + 6 \\lambda} - 4 \\lambda \\right) \\lambda}{1 + \\frac{ - \\lambda^{2}}{1 + \\frac{ - 4 \\lambda^{2}}{1 + \\lambda} + 5 \\lambda} + \\frac{ - \\left( \\frac{ - \\left( \\frac{2 \\lambda^{2}}{1 + \\lambda} - 4 \\lambda \\right) \\lambda}{1 + \\frac{ - 4 \\lambda^{2}}{1 + \\lambda} + 5 \\lambda} - 4 \\lambda \\right)^{2}}{1 + \\frac{ - \\left( \\frac{2 \\lambda^{2}}{1 + \\lambda} - 4 \\lambda \\right)^{2}}{1 + \\frac{ - 4 \\lambda^{2}}{1 + \\lambda} + 5 \\lambda} + \\frac{ - \\lambda^{2}}{1 + \\lambda} + 6 \\lambda} + 6 \\lambda} - 4 \\lambda}{1 + \\frac{ - \\lambda^{2}}{1 + \\frac{ - \\left( \\frac{2 \\lambda^{2}}{1 + \\lambda} - 4 \\lambda \\right)^{2}}{1 + \\frac{ - 4 \\lambda^{2}}{1 + \\lambda} + 5 \\lambda} + \\frac{ - \\lambda^{2}}{1 + \\lambda} + 6 \\lambda} + \\frac{ - \\left( \\frac{ - \\left( \\frac{ - \\left( \\frac{2 \\lambda^{2}}{1 + \\lambda} - 4 \\lambda \\right) \\lambda}{1 + \\frac{ - 4 \\lambda^{2}}{1 + \\lambda} + 5 \\lambda} - 4 \\lambda \\right) \\lambda}{1 + \\frac{ - \\left( \\frac{2 \\lambda^{2}}{1 + \\lambda} - 4 \\lambda \\right)^{2}}{1 + \\frac{ - 4 \\lambda^{2}}{1 + \\lambda} + 5 \\lambda} + \\frac{ - \\lambda^{2}}{1 + \\lambda} + 6 \\lambda} - 4 \\lambda \\right)^{2}}{1 + \\frac{ - \\lambda^{2}}{1 + \\frac{ - 4 \\lambda^{2}}{1 + \\lambda} + 5 \\lambda} + \\frac{ - \\left( \\frac{ - \\left( \\frac{2 \\lambda^{2}}{1 + \\lambda} - 4 \\lambda \\right) \\lambda}{1 + \\frac{ - 4 \\lambda^{2}}{1 + \\lambda} + 5 \\lambda} - 4 \\lambda \\right)^{2}}{1 + \\frac{ - \\left( \\frac{2 \\lambda^{2}}{1 + \\lambda} - 4 \\lambda \\right)^{2}}{1 + \\frac{ - 4 \\lambda^{2}}{1 + \\lambda} + 5 \\lambda} + \\frac{ - \\lambda^{2}}{1 + \\lambda} + 6 \\lambda} + 6 \\lambda} + 6 \\lambda} & 1 & 0 & 0 \\\\\n",
       "0 & 0 & 0 & 0 & \\frac{\\lambda}{1 + \\frac{ - \\lambda^{2}}{1 + \\frac{ - \\left( \\frac{2 \\lambda^{2}}{1 + \\lambda} - 4 \\lambda \\right)^{2}}{1 + \\frac{ - 4 \\lambda^{2}}{1 + \\lambda} + 5 \\lambda} + \\frac{ - \\lambda^{2}}{1 + \\lambda} + 6 \\lambda} + \\frac{ - \\left( \\frac{ - \\left( \\frac{ - \\left( \\frac{2 \\lambda^{2}}{1 + \\lambda} - 4 \\lambda \\right) \\lambda}{1 + \\frac{ - 4 \\lambda^{2}}{1 + \\lambda} + 5 \\lambda} - 4 \\lambda \\right) \\lambda}{1 + \\frac{ - \\left( \\frac{2 \\lambda^{2}}{1 + \\lambda} - 4 \\lambda \\right)^{2}}{1 + \\frac{ - 4 \\lambda^{2}}{1 + \\lambda} + 5 \\lambda} + \\frac{ - \\lambda^{2}}{1 + \\lambda} + 6 \\lambda} - 4 \\lambda \\right)^{2}}{1 + \\frac{ - \\lambda^{2}}{1 + \\frac{ - 4 \\lambda^{2}}{1 + \\lambda} + 5 \\lambda} + \\frac{ - \\left( \\frac{ - \\left( \\frac{2 \\lambda^{2}}{1 + \\lambda} - 4 \\lambda \\right) \\lambda}{1 + \\frac{ - 4 \\lambda^{2}}{1 + \\lambda} + 5 \\lambda} - 4 \\lambda \\right)^{2}}{1 + \\frac{ - \\left( \\frac{2 \\lambda^{2}}{1 + \\lambda} - 4 \\lambda \\right)^{2}}{1 + \\frac{ - 4 \\lambda^{2}}{1 + \\lambda} + 5 \\lambda} + \\frac{ - \\lambda^{2}}{1 + \\lambda} + 6 \\lambda} + 6 \\lambda} + 6 \\lambda} & \\frac{\\frac{ - \\left( \\frac{ - \\left( \\frac{ - \\left( \\frac{ - \\left( \\frac{2 \\lambda^{2}}{1 + \\lambda} - 4 \\lambda \\right) \\lambda}{1 + \\frac{ - 4 \\lambda^{2}}{1 + \\lambda} + 5 \\lambda} - 4 \\lambda \\right) \\lambda}{1 + \\frac{ - \\left( \\frac{2 \\lambda^{2}}{1 + \\lambda} - 4 \\lambda \\right)^{2}}{1 + \\frac{ - 4 \\lambda^{2}}{1 + \\lambda} + 5 \\lambda} + \\frac{ - \\lambda^{2}}{1 + \\lambda} + 6 \\lambda} - 4 \\lambda \\right) \\lambda}{1 + \\frac{ - \\lambda^{2}}{1 + \\frac{ - 4 \\lambda^{2}}{1 + \\lambda} + 5 \\lambda} + \\frac{ - \\left( \\frac{ - \\left( \\frac{2 \\lambda^{2}}{1 + \\lambda} - 4 \\lambda \\right) \\lambda}{1 + \\frac{ - 4 \\lambda^{2}}{1 + \\lambda} + 5 \\lambda} - 4 \\lambda \\right)^{2}}{1 + \\frac{ - \\left( \\frac{2 \\lambda^{2}}{1 + \\lambda} - 4 \\lambda \\right)^{2}}{1 + \\frac{ - 4 \\lambda^{2}}{1 + \\lambda} + 5 \\lambda} + \\frac{ - \\lambda^{2}}{1 + \\lambda} + 6 \\lambda} + 6 \\lambda} - 4 \\lambda \\right) \\lambda}{1 + \\frac{ - \\lambda^{2}}{1 + \\frac{ - \\left( \\frac{2 \\lambda^{2}}{1 + \\lambda} - 4 \\lambda \\right)^{2}}{1 + \\frac{ - 4 \\lambda^{2}}{1 + \\lambda} + 5 \\lambda} + \\frac{ - \\lambda^{2}}{1 + \\lambda} + 6 \\lambda} + \\frac{ - \\left( \\frac{ - \\left( \\frac{ - \\left( \\frac{2 \\lambda^{2}}{1 + \\lambda} - 4 \\lambda \\right) \\lambda}{1 + \\frac{ - 4 \\lambda^{2}}{1 + \\lambda} + 5 \\lambda} - 4 \\lambda \\right) \\lambda}{1 + \\frac{ - \\left( \\frac{2 \\lambda^{2}}{1 + \\lambda} - 4 \\lambda \\right)^{2}}{1 + \\frac{ - 4 \\lambda^{2}}{1 + \\lambda} + 5 \\lambda} + \\frac{ - \\lambda^{2}}{1 + \\lambda} + 6 \\lambda} - 4 \\lambda \\right)^{2}}{1 + \\frac{ - \\lambda^{2}}{1 + \\frac{ - 4 \\lambda^{2}}{1 + \\lambda} + 5 \\lambda} + \\frac{ - \\left( \\frac{ - \\left( \\frac{2 \\lambda^{2}}{1 + \\lambda} - 4 \\lambda \\right) \\lambda}{1 + \\frac{ - 4 \\lambda^{2}}{1 + \\lambda} + 5 \\lambda} - 4 \\lambda \\right)^{2}}{1 + \\frac{ - \\left( \\frac{2 \\lambda^{2}}{1 + \\lambda} - 4 \\lambda \\right)^{2}}{1 + \\frac{ - 4 \\lambda^{2}}{1 + \\lambda} + 5 \\lambda} + \\frac{ - \\lambda^{2}}{1 + \\lambda} + 6 \\lambda} + 6 \\lambda} + 6 \\lambda} - 4 \\lambda}{1 + \\frac{ - \\lambda^{2}}{1 + \\frac{ - \\lambda^{2}}{1 + \\frac{ - 4 \\lambda^{2}}{1 + \\lambda} + 5 \\lambda} + \\frac{ - \\left( \\frac{ - \\left( \\frac{2 \\lambda^{2}}{1 + \\lambda} - 4 \\lambda \\right) \\lambda}{1 + \\frac{ - 4 \\lambda^{2}}{1 + \\lambda} + 5 \\lambda} - 4 \\lambda \\right)^{2}}{1 + \\frac{ - \\left( \\frac{2 \\lambda^{2}}{1 + \\lambda} - 4 \\lambda \\right)^{2}}{1 + \\frac{ - 4 \\lambda^{2}}{1 + \\lambda} + 5 \\lambda} + \\frac{ - \\lambda^{2}}{1 + \\lambda} + 6 \\lambda} + 6 \\lambda} + \\frac{ - \\left( \\frac{ - \\left( \\frac{ - \\left( \\frac{ - \\left( \\frac{2 \\lambda^{2}}{1 + \\lambda} - 4 \\lambda \\right) \\lambda}{1 + \\frac{ - 4 \\lambda^{2}}{1 + \\lambda} + 5 \\lambda} - 4 \\lambda \\right) \\lambda}{1 + \\frac{ - \\left( \\frac{2 \\lambda^{2}}{1 + \\lambda} - 4 \\lambda \\right)^{2}}{1 + \\frac{ - 4 \\lambda^{2}}{1 + \\lambda} + 5 \\lambda} + \\frac{ - \\lambda^{2}}{1 + \\lambda} + 6 \\lambda} - 4 \\lambda \\right) \\lambda}{1 + \\frac{ - \\lambda^{2}}{1 + \\frac{ - 4 \\lambda^{2}}{1 + \\lambda} + 5 \\lambda} + \\frac{ - \\left( \\frac{ - \\left( \\frac{2 \\lambda^{2}}{1 + \\lambda} - 4 \\lambda \\right) \\lambda}{1 + \\frac{ - 4 \\lambda^{2}}{1 + \\lambda} + 5 \\lambda} - 4 \\lambda \\right)^{2}}{1 + \\frac{ - \\left( \\frac{2 \\lambda^{2}}{1 + \\lambda} - 4 \\lambda \\right)^{2}}{1 + \\frac{ - 4 \\lambda^{2}}{1 + \\lambda} + 5 \\lambda} + \\frac{ - \\lambda^{2}}{1 + \\lambda} + 6 \\lambda} + 6 \\lambda} - 4 \\lambda \\right)^{2}}{1 + \\frac{ - \\lambda^{2}}{1 + \\frac{ - \\left( \\frac{2 \\lambda^{2}}{1 + \\lambda} - 4 \\lambda \\right)^{2}}{1 + \\frac{ - 4 \\lambda^{2}}{1 + \\lambda} + 5 \\lambda} + \\frac{ - \\lambda^{2}}{1 + \\lambda} + 6 \\lambda} + \\frac{ - \\left( \\frac{ - \\left( \\frac{ - \\left( \\frac{2 \\lambda^{2}}{1 + \\lambda} - 4 \\lambda \\right) \\lambda}{1 + \\frac{ - 4 \\lambda^{2}}{1 + \\lambda} + 5 \\lambda} - 4 \\lambda \\right) \\lambda}{1 + \\frac{ - \\left( \\frac{2 \\lambda^{2}}{1 + \\lambda} - 4 \\lambda \\right)^{2}}{1 + \\frac{ - 4 \\lambda^{2}}{1 + \\lambda} + 5 \\lambda} + \\frac{ - \\lambda^{2}}{1 + \\lambda} + 6 \\lambda} - 4 \\lambda \\right)^{2}}{1 + \\frac{ - \\lambda^{2}}{1 + \\frac{ - 4 \\lambda^{2}}{1 + \\lambda} + 5 \\lambda} + \\frac{ - \\left( \\frac{ - \\left( \\frac{2 \\lambda^{2}}{1 + \\lambda} - 4 \\lambda \\right) \\lambda}{1 + \\frac{ - 4 \\lambda^{2}}{1 + \\lambda} + 5 \\lambda} - 4 \\lambda \\right)^{2}}{1 + \\frac{ - \\left( \\frac{2 \\lambda^{2}}{1 + \\lambda} - 4 \\lambda \\right)^{2}}{1 + \\frac{ - 4 \\lambda^{2}}{1 + \\lambda} + 5 \\lambda} + \\frac{ - \\lambda^{2}}{1 + \\lambda} + 6 \\lambda} + 6 \\lambda} + 6 \\lambda} + 6 \\lambda} & 1 & 0 \\\\\n",
       "0 & 0 & 0 & 0 & 0 & \\frac{\\lambda}{1 + \\frac{ - \\lambda^{2}}{1 + \\frac{ - \\lambda^{2}}{1 + \\frac{ - 4 \\lambda^{2}}{1 + \\lambda} + 5 \\lambda} + \\frac{ - \\left( \\frac{ - \\left( \\frac{2 \\lambda^{2}}{1 + \\lambda} - 4 \\lambda \\right) \\lambda}{1 + \\frac{ - 4 \\lambda^{2}}{1 + \\lambda} + 5 \\lambda} - 4 \\lambda \\right)^{2}}{1 + \\frac{ - \\left( \\frac{2 \\lambda^{2}}{1 + \\lambda} - 4 \\lambda \\right)^{2}}{1 + \\frac{ - 4 \\lambda^{2}}{1 + \\lambda} + 5 \\lambda} + \\frac{ - \\lambda^{2}}{1 + \\lambda} + 6 \\lambda} + 6 \\lambda} + \\frac{ - \\left( \\frac{ - \\left( \\frac{ - \\left( \\frac{ - \\left( \\frac{2 \\lambda^{2}}{1 + \\lambda} - 4 \\lambda \\right) \\lambda}{1 + \\frac{ - 4 \\lambda^{2}}{1 + \\lambda} + 5 \\lambda} - 4 \\lambda \\right) \\lambda}{1 + \\frac{ - \\left( \\frac{2 \\lambda^{2}}{1 + \\lambda} - 4 \\lambda \\right)^{2}}{1 + \\frac{ - 4 \\lambda^{2}}{1 + \\lambda} + 5 \\lambda} + \\frac{ - \\lambda^{2}}{1 + \\lambda} + 6 \\lambda} - 4 \\lambda \\right) \\lambda}{1 + \\frac{ - \\lambda^{2}}{1 + \\frac{ - 4 \\lambda^{2}}{1 + \\lambda} + 5 \\lambda} + \\frac{ - \\left( \\frac{ - \\left( \\frac{2 \\lambda^{2}}{1 + \\lambda} - 4 \\lambda \\right) \\lambda}{1 + \\frac{ - 4 \\lambda^{2}}{1 + \\lambda} + 5 \\lambda} - 4 \\lambda \\right)^{2}}{1 + \\frac{ - \\left( \\frac{2 \\lambda^{2}}{1 + \\lambda} - 4 \\lambda \\right)^{2}}{1 + \\frac{ - 4 \\lambda^{2}}{1 + \\lambda} + 5 \\lambda} + \\frac{ - \\lambda^{2}}{1 + \\lambda} + 6 \\lambda} + 6 \\lambda} - 4 \\lambda \\right)^{2}}{1 + \\frac{ - \\lambda^{2}}{1 + \\frac{ - \\left( \\frac{2 \\lambda^{2}}{1 + \\lambda} - 4 \\lambda \\right)^{2}}{1 + \\frac{ - 4 \\lambda^{2}}{1 + \\lambda} + 5 \\lambda} + \\frac{ - \\lambda^{2}}{1 + \\lambda} + 6 \\lambda} + \\frac{ - \\left( \\frac{ - \\left( \\frac{ - \\left( \\frac{2 \\lambda^{2}}{1 + \\lambda} - 4 \\lambda \\right) \\lambda}{1 + \\frac{ - 4 \\lambda^{2}}{1 + \\lambda} + 5 \\lambda} - 4 \\lambda \\right) \\lambda}{1 + \\frac{ - \\left( \\frac{2 \\lambda^{2}}{1 + \\lambda} - 4 \\lambda \\right)^{2}}{1 + \\frac{ - 4 \\lambda^{2}}{1 + \\lambda} + 5 \\lambda} + \\frac{ - \\lambda^{2}}{1 + \\lambda} + 6 \\lambda} - 4 \\lambda \\right)^{2}}{1 + \\frac{ - \\lambda^{2}}{1 + \\frac{ - 4 \\lambda^{2}}{1 + \\lambda} + 5 \\lambda} + \\frac{ - \\left( \\frac{ - \\left( \\frac{2 \\lambda^{2}}{1 + \\lambda} - 4 \\lambda \\right) \\lambda}{1 + \\frac{ - 4 \\lambda^{2}}{1 + \\lambda} + 5 \\lambda} - 4 \\lambda \\right)^{2}}{1 + \\frac{ - \\left( \\frac{2 \\lambda^{2}}{1 + \\lambda} - 4 \\lambda \\right)^{2}}{1 + \\frac{ - 4 \\lambda^{2}}{1 + \\lambda} + 5 \\lambda} + \\frac{ - \\lambda^{2}}{1 + \\lambda} + 6 \\lambda} + 6 \\lambda} + 6 \\lambda} + 6 \\lambda} & \\frac{\\frac{ - \\left( \\frac{ - \\left( \\frac{ - \\left( \\frac{ - \\left( \\frac{ - \\left( \\frac{2 \\lambda^{2}}{1 + \\lambda} - 4 \\lambda \\right) \\lambda}{1 + \\frac{ - 4 \\lambda^{2}}{1 + \\lambda} + 5 \\lambda} - 4 \\lambda \\right) \\lambda}{1 + \\frac{ - \\left( \\frac{2 \\lambda^{2}}{1 + \\lambda} - 4 \\lambda \\right)^{2}}{1 + \\frac{ - 4 \\lambda^{2}}{1 + \\lambda} + 5 \\lambda} + \\frac{ - \\lambda^{2}}{1 + \\lambda} + 6 \\lambda} - 4 \\lambda \\right) \\lambda}{1 + \\frac{ - \\lambda^{2}}{1 + \\frac{ - 4 \\lambda^{2}}{1 + \\lambda} + 5 \\lambda} + \\frac{ - \\left( \\frac{ - \\left( \\frac{2 \\lambda^{2}}{1 + \\lambda} - 4 \\lambda \\right) \\lambda}{1 + \\frac{ - 4 \\lambda^{2}}{1 + \\lambda} + 5 \\lambda} - 4 \\lambda \\right)^{2}}{1 + \\frac{ - \\left( \\frac{2 \\lambda^{2}}{1 + \\lambda} - 4 \\lambda \\right)^{2}}{1 + \\frac{ - 4 \\lambda^{2}}{1 + \\lambda} + 5 \\lambda} + \\frac{ - \\lambda^{2}}{1 + \\lambda} + 6 \\lambda} + 6 \\lambda} - 4 \\lambda \\right) \\lambda}{1 + \\frac{ - \\lambda^{2}}{1 + \\frac{ - \\left( \\frac{2 \\lambda^{2}}{1 + \\lambda} - 4 \\lambda \\right)^{2}}{1 + \\frac{ - 4 \\lambda^{2}}{1 + \\lambda} + 5 \\lambda} + \\frac{ - \\lambda^{2}}{1 + \\lambda} + 6 \\lambda} + \\frac{ - \\left( \\frac{ - \\left( \\frac{ - \\left( \\frac{2 \\lambda^{2}}{1 + \\lambda} - 4 \\lambda \\right) \\lambda}{1 + \\frac{ - 4 \\lambda^{2}}{1 + \\lambda} + 5 \\lambda} - 4 \\lambda \\right) \\lambda}{1 + \\frac{ - \\left( \\frac{2 \\lambda^{2}}{1 + \\lambda} - 4 \\lambda \\right)^{2}}{1 + \\frac{ - 4 \\lambda^{2}}{1 + \\lambda} + 5 \\lambda} + \\frac{ - \\lambda^{2}}{1 + \\lambda} + 6 \\lambda} - 4 \\lambda \\right)^{2}}{1 + \\frac{ - \\lambda^{2}}{1 + \\frac{ - 4 \\lambda^{2}}{1 + \\lambda} + 5 \\lambda} + \\frac{ - \\left( \\frac{ - \\left( \\frac{2 \\lambda^{2}}{1 + \\lambda} - 4 \\lambda \\right) \\lambda}{1 + \\frac{ - 4 \\lambda^{2}}{1 + \\lambda} + 5 \\lambda} - 4 \\lambda \\right)^{2}}{1 + \\frac{ - \\left( \\frac{2 \\lambda^{2}}{1 + \\lambda} - 4 \\lambda \\right)^{2}}{1 + \\frac{ - 4 \\lambda^{2}}{1 + \\lambda} + 5 \\lambda} + \\frac{ - \\lambda^{2}}{1 + \\lambda} + 6 \\lambda} + 6 \\lambda} + 6 \\lambda} - 4 \\lambda \\right) \\lambda}{1 + \\frac{ - \\lambda^{2}}{1 + \\frac{ - \\lambda^{2}}{1 + \\frac{ - 4 \\lambda^{2}}{1 + \\lambda} + 5 \\lambda} + \\frac{ - \\left( \\frac{ - \\left( \\frac{2 \\lambda^{2}}{1 + \\lambda} - 4 \\lambda \\right) \\lambda}{1 + \\frac{ - 4 \\lambda^{2}}{1 + \\lambda} + 5 \\lambda} - 4 \\lambda \\right)^{2}}{1 + \\frac{ - \\left( \\frac{2 \\lambda^{2}}{1 + \\lambda} - 4 \\lambda \\right)^{2}}{1 + \\frac{ - 4 \\lambda^{2}}{1 + \\lambda} + 5 \\lambda} + \\frac{ - \\lambda^{2}}{1 + \\lambda} + 6 \\lambda} + 6 \\lambda} + \\frac{ - \\left( \\frac{ - \\left( \\frac{ - \\left( \\frac{ - \\left( \\frac{2 \\lambda^{2}}{1 + \\lambda} - 4 \\lambda \\right) \\lambda}{1 + \\frac{ - 4 \\lambda^{2}}{1 + \\lambda} + 5 \\lambda} - 4 \\lambda \\right) \\lambda}{1 + \\frac{ - \\left( \\frac{2 \\lambda^{2}}{1 + \\lambda} - 4 \\lambda \\right)^{2}}{1 + \\frac{ - 4 \\lambda^{2}}{1 + \\lambda} + 5 \\lambda} + \\frac{ - \\lambda^{2}}{1 + \\lambda} + 6 \\lambda} - 4 \\lambda \\right) \\lambda}{1 + \\frac{ - \\lambda^{2}}{1 + \\frac{ - 4 \\lambda^{2}}{1 + \\lambda} + 5 \\lambda} + \\frac{ - \\left( \\frac{ - \\left( \\frac{2 \\lambda^{2}}{1 + \\lambda} - 4 \\lambda \\right) \\lambda}{1 + \\frac{ - 4 \\lambda^{2}}{1 + \\lambda} + 5 \\lambda} - 4 \\lambda \\right)^{2}}{1 + \\frac{ - \\left( \\frac{2 \\lambda^{2}}{1 + \\lambda} - 4 \\lambda \\right)^{2}}{1 + \\frac{ - 4 \\lambda^{2}}{1 + \\lambda} + 5 \\lambda} + \\frac{ - \\lambda^{2}}{1 + \\lambda} + 6 \\lambda} + 6 \\lambda} - 4 \\lambda \\right)^{2}}{1 + \\frac{ - \\lambda^{2}}{1 + \\frac{ - \\left( \\frac{2 \\lambda^{2}}{1 + \\lambda} - 4 \\lambda \\right)^{2}}{1 + \\frac{ - 4 \\lambda^{2}}{1 + \\lambda} + 5 \\lambda} + \\frac{ - \\lambda^{2}}{1 + \\lambda} + 6 \\lambda} + \\frac{ - \\left( \\frac{ - \\left( \\frac{ - \\left( \\frac{2 \\lambda^{2}}{1 + \\lambda} - 4 \\lambda \\right) \\lambda}{1 + \\frac{ - 4 \\lambda^{2}}{1 + \\lambda} + 5 \\lambda} - 4 \\lambda \\right) \\lambda}{1 + \\frac{ - \\left( \\frac{2 \\lambda^{2}}{1 + \\lambda} - 4 \\lambda \\right)^{2}}{1 + \\frac{ - 4 \\lambda^{2}}{1 + \\lambda} + 5 \\lambda} + \\frac{ - \\lambda^{2}}{1 + \\lambda} + 6 \\lambda} - 4 \\lambda \\right)^{2}}{1 + \\frac{ - \\lambda^{2}}{1 + \\frac{ - 4 \\lambda^{2}}{1 + \\lambda} + 5 \\lambda} + \\frac{ - \\left( \\frac{ - \\left( \\frac{2 \\lambda^{2}}{1 + \\lambda} - 4 \\lambda \\right) \\lambda}{1 + \\frac{ - 4 \\lambda^{2}}{1 + \\lambda} + 5 \\lambda} - 4 \\lambda \\right)^{2}}{1 + \\frac{ - \\left( \\frac{2 \\lambda^{2}}{1 + \\lambda} - 4 \\lambda \\right)^{2}}{1 + \\frac{ - 4 \\lambda^{2}}{1 + \\lambda} + 5 \\lambda} + \\frac{ - \\lambda^{2}}{1 + \\lambda} + 6 \\lambda} + 6 \\lambda} + 6 \\lambda} + 6 \\lambda} - 2 \\lambda}{1 + \\frac{ - \\lambda^{2}}{1 + \\frac{ - \\lambda^{2}}{1 + \\frac{ - \\left( \\frac{2 \\lambda^{2}}{1 + \\lambda} - 4 \\lambda \\right)^{2}}{1 + \\frac{ - 4 \\lambda^{2}}{1 + \\lambda} + 5 \\lambda} + \\frac{ - \\lambda^{2}}{1 + \\lambda} + 6 \\lambda} + \\frac{ - \\left( \\frac{ - \\left( \\frac{ - \\left( \\frac{2 \\lambda^{2}}{1 + \\lambda} - 4 \\lambda \\right) \\lambda}{1 + \\frac{ - 4 \\lambda^{2}}{1 + \\lambda} + 5 \\lambda} - 4 \\lambda \\right) \\lambda}{1 + \\frac{ - \\left( \\frac{2 \\lambda^{2}}{1 + \\lambda} - 4 \\lambda \\right)^{2}}{1 + \\frac{ - 4 \\lambda^{2}}{1 + \\lambda} + 5 \\lambda} + \\frac{ - \\lambda^{2}}{1 + \\lambda} + 6 \\lambda} - 4 \\lambda \\right)^{2}}{1 + \\frac{ - \\lambda^{2}}{1 + \\frac{ - 4 \\lambda^{2}}{1 + \\lambda} + 5 \\lambda} + \\frac{ - \\left( \\frac{ - \\left( \\frac{2 \\lambda^{2}}{1 + \\lambda} - 4 \\lambda \\right) \\lambda}{1 + \\frac{ - 4 \\lambda^{2}}{1 + \\lambda} + 5 \\lambda} - 4 \\lambda \\right)^{2}}{1 + \\frac{ - \\left( \\frac{2 \\lambda^{2}}{1 + \\lambda} - 4 \\lambda \\right)^{2}}{1 + \\frac{ - 4 \\lambda^{2}}{1 + \\lambda} + 5 \\lambda} + \\frac{ - \\lambda^{2}}{1 + \\lambda} + 6 \\lambda} + 6 \\lambda} + 6 \\lambda} + \\frac{ - \\left( \\frac{ - \\left( \\frac{ - \\left( \\frac{ - \\left( \\frac{ - \\left( \\frac{2 \\lambda^{2}}{1 + \\lambda} - 4 \\lambda \\right) \\lambda}{1 + \\frac{ - 4 \\lambda^{2}}{1 + \\lambda} + 5 \\lambda} - 4 \\lambda \\right) \\lambda}{1 + \\frac{ - \\left( \\frac{2 \\lambda^{2}}{1 + \\lambda} - 4 \\lambda \\right)^{2}}{1 + \\frac{ - 4 \\lambda^{2}}{1 + \\lambda} + 5 \\lambda} + \\frac{ - \\lambda^{2}}{1 + \\lambda} + 6 \\lambda} - 4 \\lambda \\right) \\lambda}{1 + \\frac{ - \\lambda^{2}}{1 + \\frac{ - 4 \\lambda^{2}}{1 + \\lambda} + 5 \\lambda} + \\frac{ - \\left( \\frac{ - \\left( \\frac{2 \\lambda^{2}}{1 + \\lambda} - 4 \\lambda \\right) \\lambda}{1 + \\frac{ - 4 \\lambda^{2}}{1 + \\lambda} + 5 \\lambda} - 4 \\lambda \\right)^{2}}{1 + \\frac{ - \\left( \\frac{2 \\lambda^{2}}{1 + \\lambda} - 4 \\lambda \\right)^{2}}{1 + \\frac{ - 4 \\lambda^{2}}{1 + \\lambda} + 5 \\lambda} + \\frac{ - \\lambda^{2}}{1 + \\lambda} + 6 \\lambda} + 6 \\lambda} - 4 \\lambda \\right) \\lambda}{1 + \\frac{ - \\lambda^{2}}{1 + \\frac{ - \\left( \\frac{2 \\lambda^{2}}{1 + \\lambda} - 4 \\lambda \\right)^{2}}{1 + \\frac{ - 4 \\lambda^{2}}{1 + \\lambda} + 5 \\lambda} + \\frac{ - \\lambda^{2}}{1 + \\lambda} + 6 \\lambda} + \\frac{ - \\left( \\frac{ - \\left( \\frac{ - \\left( \\frac{2 \\lambda^{2}}{1 + \\lambda} - 4 \\lambda \\right) \\lambda}{1 + \\frac{ - 4 \\lambda^{2}}{1 + \\lambda} + 5 \\lambda} - 4 \\lambda \\right) \\lambda}{1 + \\frac{ - \\left( \\frac{2 \\lambda^{2}}{1 + \\lambda} - 4 \\lambda \\right)^{2}}{1 + \\frac{ - 4 \\lambda^{2}}{1 + \\lambda} + 5 \\lambda} + \\frac{ - \\lambda^{2}}{1 + \\lambda} + 6 \\lambda} - 4 \\lambda \\right)^{2}}{1 + \\frac{ - \\lambda^{2}}{1 + \\frac{ - 4 \\lambda^{2}}{1 + \\lambda} + 5 \\lambda} + \\frac{ - \\left( \\frac{ - \\left( \\frac{2 \\lambda^{2}}{1 + \\lambda} - 4 \\lambda \\right) \\lambda}{1 + \\frac{ - 4 \\lambda^{2}}{1 + \\lambda} + 5 \\lambda} - 4 \\lambda \\right)^{2}}{1 + \\frac{ - \\left( \\frac{2 \\lambda^{2}}{1 + \\lambda} - 4 \\lambda \\right)^{2}}{1 + \\frac{ - 4 \\lambda^{2}}{1 + \\lambda} + 5 \\lambda} + \\frac{ - \\lambda^{2}}{1 + \\lambda} + 6 \\lambda} + 6 \\lambda} + 6 \\lambda} - 4 \\lambda \\right)^{2}}{1 + \\frac{ - \\lambda^{2}}{1 + \\frac{ - \\lambda^{2}}{1 + \\frac{ - 4 \\lambda^{2}}{1 + \\lambda} + 5 \\lambda} + \\frac{ - \\left( \\frac{ - \\left( \\frac{2 \\lambda^{2}}{1 + \\lambda} - 4 \\lambda \\right) \\lambda}{1 + \\frac{ - 4 \\lambda^{2}}{1 + \\lambda} + 5 \\lambda} - 4 \\lambda \\right)^{2}}{1 + \\frac{ - \\left( \\frac{2 \\lambda^{2}}{1 + \\lambda} - 4 \\lambda \\right)^{2}}{1 + \\frac{ - 4 \\lambda^{2}}{1 + \\lambda} + 5 \\lambda} + \\frac{ - \\lambda^{2}}{1 + \\lambda} + 6 \\lambda} + 6 \\lambda} + \\frac{ - \\left( \\frac{ - \\left( \\frac{ - \\left( \\frac{ - \\left( \\frac{2 \\lambda^{2}}{1 + \\lambda} - 4 \\lambda \\right) \\lambda}{1 + \\frac{ - 4 \\lambda^{2}}{1 + \\lambda} + 5 \\lambda} - 4 \\lambda \\right) \\lambda}{1 + \\frac{ - \\left( \\frac{2 \\lambda^{2}}{1 + \\lambda} - 4 \\lambda \\right)^{2}}{1 + \\frac{ - 4 \\lambda^{2}}{1 + \\lambda} + 5 \\lambda} + \\frac{ - \\lambda^{2}}{1 + \\lambda} + 6 \\lambda} - 4 \\lambda \\right) \\lambda}{1 + \\frac{ - \\lambda^{2}}{1 + \\frac{ - 4 \\lambda^{2}}{1 + \\lambda} + 5 \\lambda} + \\frac{ - \\left( \\frac{ - \\left( \\frac{2 \\lambda^{2}}{1 + \\lambda} - 4 \\lambda \\right) \\lambda}{1 + \\frac{ - 4 \\lambda^{2}}{1 + \\lambda} + 5 \\lambda} - 4 \\lambda \\right)^{2}}{1 + \\frac{ - \\left( \\frac{2 \\lambda^{2}}{1 + \\lambda} - 4 \\lambda \\right)^{2}}{1 + \\frac{ - 4 \\lambda^{2}}{1 + \\lambda} + 5 \\lambda} + \\frac{ - \\lambda^{2}}{1 + \\lambda} + 6 \\lambda} + 6 \\lambda} - 4 \\lambda \\right)^{2}}{1 + \\frac{ - \\lambda^{2}}{1 + \\frac{ - \\left( \\frac{2 \\lambda^{2}}{1 + \\lambda} - 4 \\lambda \\right)^{2}}{1 + \\frac{ - 4 \\lambda^{2}}{1 + \\lambda} + 5 \\lambda} + \\frac{ - \\lambda^{2}}{1 + \\lambda} + 6 \\lambda} + \\frac{ - \\left( \\frac{ - \\left( \\frac{ - \\left( \\frac{2 \\lambda^{2}}{1 + \\lambda} - 4 \\lambda \\right) \\lambda}{1 + \\frac{ - 4 \\lambda^{2}}{1 + \\lambda} + 5 \\lambda} - 4 \\lambda \\right) \\lambda}{1 + \\frac{ - \\left( \\frac{2 \\lambda^{2}}{1 + \\lambda} - 4 \\lambda \\right)^{2}}{1 + \\frac{ - 4 \\lambda^{2}}{1 + \\lambda} + 5 \\lambda} + \\frac{ - \\lambda^{2}}{1 + \\lambda} + 6 \\lambda} - 4 \\lambda \\right)^{2}}{1 + \\frac{ - \\lambda^{2}}{1 + \\frac{ - 4 \\lambda^{2}}{1 + \\lambda} + 5 \\lambda} + \\frac{ - \\left( \\frac{ - \\left( \\frac{2 \\lambda^{2}}{1 + \\lambda} - 4 \\lambda \\right) \\lambda}{1 + \\frac{ - 4 \\lambda^{2}}{1 + \\lambda} + 5 \\lambda} - 4 \\lambda \\right)^{2}}{1 + \\frac{ - \\left( \\frac{2 \\lambda^{2}}{1 + \\lambda} - 4 \\lambda \\right)^{2}}{1 + \\frac{ - 4 \\lambda^{2}}{1 + \\lambda} + 5 \\lambda} + \\frac{ - \\lambda^{2}}{1 + \\lambda} + 6 \\lambda} + 6 \\lambda} + 6 \\lambda} + 6 \\lambda} + 5 \\lambda} & 1 \\\\\n",
       "\\end{array}\n",
       "\\right]\n",
       "\\end{equation}\n",
       " $$"
      ],
      "text/plain": [
       "8×8 Matrix{Num}:\n",
       "          1         …  0\n",
       " (-2λ) / (1.0 + λ)     0\n",
       "     λ / (1.0 + λ)     0\n",
       "          0.0          0\n",
       "          0.0          0\n",
       "          0.0       …  0\n",
       "          0.0          0\n",
       "          0.0          1"
      ]
     },
     "metadata": {},
     "output_type": "display_data"
    }
   ],
   "source": []
  }
 ],
 "metadata": {
  "kernelspec": {
   "display_name": "Julia 1.10.3",
   "language": "julia",
   "name": "julia-1.10"
  },
  "language_info": {
   "file_extension": ".jl",
   "mimetype": "application/julia",
   "name": "julia",
   "version": "1.10.3"
  }
 },
 "nbformat": 4,
 "nbformat_minor": 5
}
